WIP

src/specs/UpdateAggregationChallenge.ec
@@ -17,9 +17,22 @@ module UpdateAggregationChallenge = {
     newAggregatedOpeningAtZ <- (PurePrimops.addmod curAggregatedOpeningAtZ _6 R_MOD);
     return (newAggregationChallenge, newAggregatedOpeningAtZ);
   }
+      proc mid(queriesCommitmentPoint : int * int, currAggregatedAtZXSlot : int * int, valueAtZ : int, currAggregationChallenge : int, curAggregatedOpeningAtZ : int, v_challenge : int) : (int * int * (int * int)) option = {
+      var newAggregationChallenge, newAggregatedOpeningAtZ, mNewAggregateAtZXSlot, newAggregateAtZXSlot, ret; 
+      newAggregationChallenge <- v_challenge * currAggregationChallenge %% Constants.R;
+      mNewAggregateAtZXSlot <@ PointMulAndAddIntoDest.mid(queriesCommitmentPoint.`1, queriesCommitmentPoint.`2, newAggregationChallenge, currAggregatedAtZXSlot.`1, currAggregatedAtZXSlot.`2);
+      if (is_some mNewAggregateAtZXSlot) {
+        newAggregateAtZXSlot <- odflt (0, 0) mNewAggregateAtZXSlot;
+        newAggregatedOpeningAtZ <- (newAggregationChallenge * valueAtZ + curAggregatedOpeningAtZ) %% Constants.R;
+        ret   <- Some (newAggregationChallenge, newAggregatedOpeningAtZ, newAggregateAtZXSlot);
+      } else {
+          ret <- None;
+      }
+      return ret;
+  }
 }.
 
-lemma updateAggregationChallenge_extracted_equiv_low :
+lemma UpdateAggregationChallenge_extracted_equiv_low :
     equiv [
       Verifier_1261.usr_updateAggregationChallenge ~ UpdateAggregationChallenge.low :
       ={arg, glob UpdateAggregationChallenge} ==>
@@ -31,3 +44,33 @@ proof.
   call (pointMulAndAddIntoDest_extracted_equiv_low). wp.
   skip. rewrite /Constants.R. by progress.
 qed.
+
+lemma UpdateAggregationChallenge_mid_of_low (queriesCommitmentPoint : int * int) (currAggregatedAtZXSlot : int * int) (valueAtZ : int) (currAggregationChallenge : int) (curAggregatedOpeningAtZ : int) (v_challenge : int) (queriesCommitmentPoint_addr valueAtZ_addr : uint256) (memory0 : MemoryMap.mem) : equiv [
+    UpdateAggregationChallenge.low ~ UpdateAggregationChallenge.mid :
+    Primops.memory{1} = memory0 /\
+    arg{1} = (queriesCommitmentPoint_addr, valueAtZ_addr, W256.of_int currAggregationChallenge, W256.of_int curAggregatedOpeningAtZ) /\
+    arg{2} = (queriesCommitmentPoint, currAggregatedAtZXSlot, valueAtZ, currAggregationChallenge, curAggregatedOpeningAtZ, v_challenge) /\
+    PurePrimops.mload memory0 STATE_V_SLOT = W256.of_int v_challenge /\
+    PurePrimops.mload memory0 valueAtZ_addr = W256.of_int valueAtZ /\
+    PurePrimops.mload memory0 queriesCommitmentPoint_addr = W256.of_int queriesCommitmentPoint.`1 /\
+    PurePrimops.mload memory0 (queriesCommitmentPoint_addr + W256.of_int 32) = W256.of_int queriesCommitmentPoint.`2 /\
+    PurePrimops.mload memory0 AGGREGATED_AT_Z_X_SLOT = W256.of_int currAggregatedAtZXSlot.`1 /\
+    PurePrimops.mload memory0 (AGGREGATED_AT_Z_X_SLOT + W256.of_int 32) = W256.of_int currAggregatedAtZXSlot.`2 
+      ==>
+      (res{2} = None) \/
+      (
+        exists (newAggregationChallenge newAggregatedOpeningAtZ : int) (newAggregateAtZXSlot : int * int),
+        newAggregationChallenge = v_challenge * currAggregationChallenge %% Constants.R /\
+        newAggregatedOpeningAtZ = (v_challenge * currAggregationChallenge * valueAtZ + curAggregatedOpeningAtZ) %% Constants.R /\
+        res{2} = Some (newAggregationChallenge, newAggregatedOpeningAtZ, newAggregateAtZXSlot))
+    ]. proof.
+        proc. inline mload. wp. sp.
+
+        exists* newAggregationChallenge{2}.
+        elim*=> val_newAggregationChallenge.
+
+        exists* Primops.memory{1}.
+        elim*=>memory1.
+    
+        call (PointMulAndAddIntoDest_mid_of_low queriesCommitmentPoint.`1 queriesCommitmentPoint.`2 currAggregatedAtZXSlot.`1 currAggregatedAtZXSlot.`2 val_newAggregationChallenge queriesCommitmentPoint_addr AGGREGATED_AT_Z_X_SLOT memory1). skip. progress.
+    
